deprecated/decl @ 5.25/prop_typing.v
@@ -1,0 +1,919 @@
+Require Import Coq.Program.Equality.
+Require Import Program.Tactics.
+Require Import Lia.
+Require Import Metalib.Metatheory.
+
+Require Import decl.notations.
+Require Import decl.prop_basic.
+Require Import decl.prop_subtyping.
+Require Import ln_utils.
+
+
+Definition wf_dom : forall {E}, ⊢ E -> atoms.
+Proof.
+  intros.
+  set (x := dom E). exact x.
+Defined.
+
+
+Ltac gather_atoms ::=
+  let A := gather_atoms_with (fun x : vars => x) in
+  let B := gather_atoms_with (fun x : var => {{ x }}) in
+  let C := gather_atoms_with (fun x : denv => dom x) in
+  let D1 := gather_atoms_with (fun x => ftv_in_dtyp x) in
+  let D2 := gather_atoms_with (fun x => fstv_in_dtyp x) in
+  (* let D3 := gather_atoms_with (fun x => fv_typ_in_binding x) in *)
+  (* let D4 := gather_atoms_with (fun x => fv_exp_in_exp x) in *)
+  constr:(A \u B \u C \u D1 \u D2).
+
+(* Ltac apply_fresh_base_fixed H gather_vars atom_name :=
+  let L := gather_vars in
+  let L := beautify_fset L in
+  let x := fresh atom_name in
+  pick fresh x excluding L and apply H. *) 
+
+(* 
+
+Tactic Notation "pick" "fresh" ident(x) "and" "apply" constr(H) "for" "weakening" :=
+  apply_fresh_base_fixed H gather_for_weakening x. *)
+
+
+Hint Constructors dwf_typ: core.
+Hint Constructors dwf_env: core.
+Hint Constructors dwf_typ_s: core.
+
+
+
+Lemma dwf_typ_weakening : forall E1 E2 E3 T, 
+  E1 ++ E3 ⊢ T ->
+  E1 ++ E2 ++ E3 ⊢ T.
+Proof.
+  intros.
+  dependent induction H; auto.
+  - eapply dwftyp_all with (L:=L `union` dom (E1 ++ E2 ++ E3));
+    intros; inst_cofinites_with X.
+    + auto.
+    + replace (X ~ dbind_tvar_empty ++ E1 ++ E2 ++ E3) with ((X ~ dbind_tvar_empty ++ E1) ++ E2 ++ E3) by auto.
+    eapply H1; eauto.
+Qed.
+
+Corollary dwf_typ_weakening_cons : forall E X b T,
+  E ⊢ T ->
+  ((X ~ b) ++ E) ⊢ T.
+Proof.
+  intros.
+  replace (X ~ b ++ E) with (nil ++ X ~ b ++ E) by auto.
+  now apply dwf_typ_weakening.
+Qed.
+  
+
+
+Lemma dwf_typ_strengthening : forall F E x T b,
+    E ++ x ~ b ++ F ⊢ T ->
+    x \notin ftv_in_dtyp T ->
+    x \notin fstv_in_dtyp T -> 
+    E ++ F ⊢ T.
+Proof.
+  intros.
+  dependent induction H; auto.
+  - induction E.
+    + inversion H. dependent destruction H2.
+      simpl in H0. apply notin_singleton_1 in H0. contradiction.
+      auto.
+    + destruct a. inversion H.
+      * dependent destruction H2. auto.
+      * simpl. apply dwf_typ_weakening_cons; auto.
+  - induction E.
+    + inversion H. dependent destruction H2.
+      * simpl in H1. apply notin_singleton_1 in H1. contradiction.
+      * auto.
+    + destruct a. inversion H.
+      * dependent destruction H2. auto.
+      * simpl. apply dwf_typ_weakening_cons; auto.
+  - simpl in *. constructor.
+    + apply notin_union_1 in H1.
+      eauto.
+    + apply notin_union_2 in H1.
+      eauto.
+  - simpl in *.
+    apply dwftyp_all with (L:=L `union` singleton x); intros; inst_cofinites_with X.
+    + auto. 
+    + replace (X ~ dbind_tvar_empty ++ E ++ F) with ((X ~ dbind_tvar_empty ++ E)++ F) by auto. eapply H1 with (x:=x) (b:=b); auto.
+    rewrite ftv_in_dtyp_open_dtyp_wrt_dtyp_upper; auto.
+    rewrite fstv_in_dtyp_open_dtyp_wrt_dtyp_upper; auto. 
+  - simpl in *. eauto.
+  - simpl in *. eauto.
+Qed.
+
+
+
+(* Lemma wft_all_inversion : forall E S T,
+  dmono_typ T ->
+  E ⊢ T ->
+  E ⊢ T2  *)
+
+(* Lemma dwf_typ_open_inv : forall E T S1 S2 n,
+  E ⊢ S1 ->
+  E ⊢ S2 ->
+  E ⊢ open_dtyp_wrt_dtyp_rec n S2 T ->
+  E ⊢ open_dtyp_wrt_dtyp_rec n S1 T.
+Proof.
+  intros. 
+  dependent induction H1; auto.
+  - destruct T; simpl in *; try solve [inversion x].
+    + econstructor.
+    + destruct (lt_eq_lt_dec n0 n).
+      * destruct s; auto. inversion x.
+      * inversion x.
+  - destruct T; simpl in *; try solve [inversion x].
+    + econstructor.
+    + destruct (lt_eq_lt_dec n0 n).
+      * destruct s; auto. inversion x.
+      * inversion x.
+  - destruct T; simpl in *; try solve [inversion x].
+    + econstructor.
+    + destruct (lt_eq_lt_dec n0 n).
+      * destruct s; auto. inversion x.
+      * inversion x.
+  - destruct T; simpl in *; try solve [inversion x].
+    + destruct (lt_eq_lt_dec n0 n).
+      * destruct s; auto. inversion x.
+      * inversion x.
+    + inversion x. subst. auto.
+  - destruct T; simpl in *; try solve [inversion x].
+    + destruct (lt_eq_lt_dec n0 n).
+      * destruct s; auto. inversion x.
+      * inversion x.
+    + inversion x. subst. auto.
+  - destruct T; simpl in *; try solve [inversion x].
+    + destruct (lt_eq_lt_dec n0 n).
+      * destruct s; auto. inversion x.
+      * inversion x.
+    + inversion x. econstructor; eauto.
+  - destruct T; simpl in *; try solve [inversion x].
+    + destruct (lt_eq_lt_dec n0 n).
+      * destruct s; auto. inversion x.
+      * inversion x.
+    + inversion x.
+      eapply dwftyp_all with (L:=L); intros; inst_cofinites_with X.
+      * admit.
+      * replace (open_dtyp_wrt_dtyp_rec (S n) S1 T ^ᵈ X) with (open_dtyp_wrt_dtyp_rec (S n) S1 (T ^ᵈ X)).
+
+        apply H1 with (S2:=S2); eauto.
+        admit.
+        admit.
+Admitted. *)
+
+Theorem dwf_typ_subst : forall E1 E2 X T1 T2, 
+  E1 ++ (X ~ dbind_tvar_empty) ++ E2 ⊢ T1 ->
+  E2 ⊢ T2 -> 
+  E1 ++ E2 ⊢ {T2 /ᵈ X} T1.
+Proof.
+  intros; dependent induction H; try solve [simpl; auto].
+  - simpl. destruct (X0 == X).
+    + replace (E1 ++ E2) with (nil ++ E1 ++ E2) by auto. 
+    apply dwf_typ_weakening; auto.
+    + econstructor. 
+      induction E1.
+      * simpl in *. inversion H; auto.
+        inversion H1. subst. contradiction. 
+      * destruct a; inversion H.
+        -- dependent destruction H1. auto.
+        -- simpl. auto.
+  - simpl. constructor.
+    induction E1.
+    + simpl in *. inversion H; auto.
+      inversion H1.
+    + destruct a; inversion H.
+      * dependent destruction H1. auto.
+      * simpl. auto.
+  - simpl. eapply dwftyp_all with (L:=L `union` singleton X).
+    + intros. inst_cofinites_with X0. 
+      admit.
+    + intros. inst_cofinites_with X0. 
+      rewrite dtyp_subst_open_comm; eauto.
+      * replace (X0 ~ dbind_tvar_empty ++ E1 ++ E2) with ((X0 ~ dbind_tvar_empty ++ E1) ++ E2) by auto. eapply H1; auto.
+Admitted.
+
+(* Theorem dwf_typ_subst_inversion : forall E X T1, 
+  E ⊢ T1 ->
+  forall T2 T3, T1 = {T2 /ᵈ X} T3 ->
+    E ⊢ T3.
+Proof.
+  intros. dependent induction H; auto.
+  - admit.
+  - admit.
+  - admit.
+  - admit.
+  - admit.
+  -
+
+  + admit.
+  + simpl in *. 
+    dependent destruction H; eauto.
+  + simpl in *.
+    apply IHT1.
+    dependent destruction H.
+    apply dwftyp_all with (L:=L); intros.
+    * admit.
+    * inst_cofinites_with X0.
+      apply IHT1.
+    appl *)
+
+
+
+(* Theorem dwf_type_subst_var: forall G1 G2 x x' A,
+  G1, x,, G2 ⊢ A ->  ⊢ G1, x',, G2 -> G1, x',, G2 ⊢ [`ᵈ x' /ᵈ x] A.
+Proof.Theorem ld_wf_type_subst_var: forall G1 G2 x x' A,
+G1, x,, G2 ⊢ A ->  ⊢ G1, x',, G2 -> G1, x',, G2 ⊢ [`ᵈ x' /ᵈ x] A.
+Proof. *)
+
+
+Lemma mono_type_order : forall T,
+  dmono_typ T -> dtyp_order T = 0.
+Proof.
+  intros. induction H; simpl; auto; lia.
+Qed. 
+
+
+(* Lemma ld_in_context_exact : 
+  forall G1 G3 x, 
+    ld_in_context x (G1,x,,G3).
+Proof.
+  intros.
+  induction G3.
+  - simpl. econstructor.
+  - simpl. apply ld_inc_there.
+    auto.
+Qed.
+
+Lemma ld_in_context_weakenning : 
+  forall G1 G2 G3 x, 
+    ld_in_context x (G1,,G3) -> ld_in_context x (G1,, G2,, G3).
+Proof.
+  intros.
+  induction G3.
+  - induction G2.
+    + auto.
+    + simpl in *. auto.
+  - simpl in *.  dependent destruction H.
+    + apply ld_inc_here.
+    + apply ld_inc_there. auto.
+Qed.
+
+Corollary ld_in_context_weakenning_single: 
+  forall G1 G3 x x', 
+    ld_in_context x (G1,,G3) -> ld_in_context x (G1, x',, G3).
+Proof.
+  intros.
+  replace (G1, x',, G3) with (G1,, (ld_ctx_nil, x'),,G3) by auto.
+  apply ld_in_context_weakenning. auto.
+Qed.
+
+
+Lemma ld_in_ctx_dom_weakenning : 
+  forall G1 G2 G3 x, 
+   x `notin` (ld_ctx_dom (G1,, G2,, G3)) -> x `notin` (ld_ctx_dom (G1,,G3)) .
+Proof.
+  intros.
+  induction G3.
+  - induction G2.
+    + auto.
+    + simpl in *. auto.
+  - simpl in *. apply notin_add_3.
+    + apply notin_add_1 in H. auto.
+    + apply IHG3. apply notin_add_2 in H. auto.
+Qed.
+
+
+
+Lemma ld_wf_type_fv: forall G t x, 
+  G ⊢ t -> x `notin` ld_ctx_dom G -> x `notin` fv_ld_type t.
+Proof.
+  intros.
+  induction H; simpl in *; auto.
+  - induction G.
+    + inversion H1.
+    + inversion H1; subst.
+      * simpl in H0. auto.
+      * inversion H. simpl in H0. apply IHG; auto.
+  - inst_cofinites_by (L `union` singleton x).
+    assert (x ∉ add x0 (ld_ctx_dom G)) by auto.
+    specialize (H1 H2). 
+    simpl in H1.
+    rewrite fv_ld_type_open_ld_type_wrt_ld_type_lower.
+    eauto.
+Qed.
+
+
+Theorem ld_wf_ctx_weakening : forall G3 G1 G2,
+  ⊢ G1 ,, G2 ,, G3 -> ⊢ G1 ,, G3.
+Proof.
+  induction G3; intros.
+  - induction G2; auto.
+    + simpl in *. apply IHG2. dependent destruction H. auto.
+  - simpl in *. dependent destruction H. econstructor. 
+    + eapply IHG3. eauto.
+    + eapply ld_in_ctx_dom_weakenning. eauto.
+Qed.
+  
+Theorem ld_wf_mtype_weakening : 
+  forall G1 G2 G3 t, 
+  ld_wf_mtype (G1 ,, G3) t -> ⊢ G1 ,, G2 ,, G3 ->
+  ld_wf_mtype (G1 ,, G2 ,, G3) t.
+Proof.
+  intros.
+  dependent induction H; eauto.
+  - econstructor; eauto. now apply ld_in_context_weakenning.
+Qed.
+
+
+Theorem ld_sub_weakening: 
+  forall G1 G2 G3 t1 t2, 
+  G1 ,, G3 ⊢ t1 <: t2 -> ⊢ G1 ,, G2 ,, G3 -> 
+  G1 ,, G2 ,, G3 ⊢ t1 <: t2.
+Proof.
+  intros.
+  dependent induction H; auto.
+  - constructor; auto. eapply ld_in_context_weakenning. auto.
+  - constructor; auto. eapply ld_wf_type_weakening; eauto.
+  - apply ld_sub_intersection_l2. auto. eapply ld_wf_type_weakening; eauto.
+  - apply ld_sub_union_r1. auto. eapply ld_wf_type_weakening; eauto.
+  - apply ld_sub_union_r2. auto. eapply ld_wf_type_weakening; eauto.
+  - eapply ld_sub_foralll with (t:=t); auto.
+    eapply ld_wf_mtype_weakening; auto.
+  - pick fresh x and apply ld_sub_forallr for weakening.
+    replace (G1,, G2,, G3, x) with (G1,, G2,, (G3, x)) by auto.
+    eapply H0; auto. constructor; auto.
+Qed.
+
+
+Theorem ld_in_context_other : forall G1 G2 x x', 
+  x <> x' -> ld_in_context x (G1, x',,G2) -> ld_in_context x (G1,,G2).
+Proof.
+  intros.
+  induction G2.
+  - simpl in *. dependent destruction H0.
+    + contradiction.
+    + auto.
+  - simpl in *. dependent destruction H0.
+    + econstructor.
+    + constructor. auto. 
+Qed.
+
+
+Theorem ld_wf_mtype_equiv_ld_wf_type_and_mono : forall G t,
+  ld_wf_mtype G t <-> G ⊢ t /\ ld_mono_type t.
+Proof.
+  intros. split; intros.
+  - dependent induction H; auto. 
+    split; intuition.
+    + split. constructor; intuition. constructor; intuition.
+    + split. constructor; intuition. constructor; intuition.
+  - inversion H. dependent induction H0; auto.
+    + dependent destruction H1. intuition.
+    + inversion H1. constructor; intuition.
+    + destruct H. inversion H0. constructor; intuition. 
+    + inversion H2.
+Qed.
+
+
+Theorem ld_wf_type_subst_var: forall G1 G2 x x' A,
+  G1, x,, G2 ⊢ A ->  ⊢ G1, x',, G2 -> G1, x',, G2 ⊢ [`ᵈ x' /ᵈ x] A.
+Proof.
+  intros.
+  dependent induction H; simpl; auto.
+  - destruct (x0 == x); subst.
+    + constructor. auto. 
+      now apply ld_in_context_exact.
+    + constructor; auto.
+      apply ld_in_context_other in H0.
+      apply ld_in_context_weakenning_single; auto.
+      auto.
+  - eapply ld_wft_forall with (L:=L `union` (singleton x) `union` (ld_ctx_dom (G1, x',, G2))).
+    intros. inst_cofinites_with x0.
+    replace (G1, x',, G2, x0) with (G1, x',, (G2, x0)) by auto.
+    replace (([`ᵈ x' /ᵈ x] t) ^ᵈ x0) with ([`ᵈ x' /ᵈ x] t ^ᵈ x0).
+    apply H0; eauto.
+    simpl. constructor; auto.
+    rewrite subst_ld_type_open_ld_type_wrt_ld_type. simpl.
+    apply notin_union_2 in H2. apply notin_union_1 in H2.
+    apply notin_singleton_1' in H2.  unfold not in H2. 
+    + destruct (x0 == x); auto.
+      * subst. contradiction.
+    + auto.
+Qed.
+
+Ltac rewrite_subst_open_var :=
+  repeat
+    match goal with 
+      | _ : _ |-  context [ ([?e /ᵈ ?x] ?A) ^^ᵈ `ᵈ ?x' ] => 
+        replace (`ᵈ x') with ([e /ᵈ x] `ᵈ x') by (apply subst_ld_type_fresh_eq; auto)
+    end; repeat rewrite <- subst_ld_type_open_ld_type_wrt_ld_type by auto.
+
+
+
+Theorem ld_wf_mtype_subst :
+  forall G1 G2 x t t', 
+    ld_mono_type t' -> ld_wf_mtype (G1, x,, G2) t -> G1 ⊢ t' ->  ld_wf_mtype (G1,, G2) ([t' /ᵈ x] t).
+Proof.
+  intros.
+  dependent induction H0.
+  - simpl. econstructor. 
+    replace (G1, x,, G2) with (G1,,(ld_ctx_nil, x),,G2) in H0 by auto. eapply ld_wf_ctx_weakening; eauto.
+  - simpl. destruct (x0 == x).
+    + apply ld_wf_mtype_equiv_ld_wf_type_and_mono. intuition.
+      replace (G1,,G2) with (G1,,G2,,ld_ctx_nil) by auto. eapply ld_wf_type_weakening. eauto.
+      simpl.  replace (G1, x,, G2) with (G1,,(ld_ctx_nil, x),,G2) in H1 by auto. eapply ld_wf_ctx_weakening; eauto.
+    + constructor.
+      * replace (G1, x,, G2) with (G1,,(ld_ctx_nil, x),,G2) in H1 by auto. eapply ld_wf_ctx_weakening; eauto.
+      * eapply ld_in_context_other; eauto.    
+  - simpl. constructor.
+    + apply IHld_wf_mtype1; auto.
+    + apply IHld_wf_mtype2; auto.  
+  - simpl. constructor.
+    + apply IHld_wf_mtype1; auto.
+    + apply IHld_wf_mtype2; auto.
+  - simpl. constructor.
+    + apply IHld_wf_mtype1; auto.
+    + apply IHld_wf_mtype2; auto.
+Qed.
+
+
+
+Theorem ld_mono_is_ld_lc : forall t, 
+  ld_mono_type t -> lc_ld_type t.
+Proof.
+  intros. induction H; auto.
+Qed.
+
+Theorem ld_wf_type_subst :
+  forall G1 G2 x t t', 
+    ld_mono_type t' -> ld_wf_type (G1, x,, G2) t -> G1 ⊢ t' ->  ld_wf_type (G1,, G2) ([t' /ᵈ x] t).
+Proof.
+  intros.
+  dependent induction H0.
+  - simpl. econstructor. 
+    replace (G1, x,, G2) with (G1,,(ld_ctx_nil, x),,G2) in H0 by auto. eapply ld_wf_ctx_weakening; eauto.
+  - simpl. destruct (x0 == x).
+    + replace (G1,,G2) with (G1,,G2,,ld_ctx_nil) by auto. eapply ld_wf_type_weakening. eauto.
+      simpl.  replace (G1, x,, G2) with (G1,,(ld_ctx_nil, x),,G2) in H1 by auto. eapply ld_wf_ctx_weakening; eauto.
+    + constructor.
+      * replace (G1, x,, G2) with (G1,,(ld_ctx_nil, x),,G2) in H1 by auto. eapply ld_wf_ctx_weakening; eauto.
+      * eapply ld_in_context_other; eauto.    
+  - simpl. constructor.
+    + apply IHld_wf_type1; auto.
+    + apply IHld_wf_type2; auto.  
+  - simpl. constructor.
+    + apply IHld_wf_type1; auto.
+    + apply IHld_wf_type2; auto.
+  - simpl. constructor.
+    + apply IHld_wf_type1; auto.
+    + apply IHld_wf_type2; auto.
+  - replace ([t' /ᵈ x] ld_t_forall t) with (ld_t_forall ([t' /ᵈ x] t)) by auto.
+    eapply ld_wft_forall with (L:=L `union` singleton x). intros. 
+    replace (([t' /ᵈ x] t) ^ᵈ x0) with ([t' /ᵈ x] t ^ᵈ x0).
+    replace (G1,, G2, x0) with (G1,, (G2, x0)) by auto. eapply H0; eauto.
+    + rewrite subst_ld_type_open_ld_type_wrt_ld_type. 
+    simpl. apply notin_union_2 in H3.
+    apply notin_singleton_1' in H3.  unfold not in H3. 
+    destruct (x0 == x).
+    * subst. contradiction.
+    * auto.
+    * now apply ld_mono_is_ld_lc.
+Qed. *)
+
+
+Inductive d_subenv : denv -> denv -> Prop := 
+| d_subenv_empty: d_subenv nil nil  
+| d_subenv_tvar : forall E1 E2 X, 
+    d_subenv E1 E2 -> 
+    d_subenv (X ~ dbind_tvar_empty  ++  E1) 
+        (X ~ dbind_tvar_empty  ++  E2)
+| d_subenv_stvar : forall E1 E2 SX, 
+    d_subenv E1 E2 -> 
+    d_subenv (SX ~ dbind_stvar_empty  ++  E1) 
+        (SX ~ dbind_stvar_empty  ++  E2)
+| d_subenv_var : forall E1 E2 x S T,
+    d_subenv E1 E2 ->
+    d_sub E2 S T ->
+    d_subenv (x ~ dbind_typ S ++ E1) 
+        (x ~ dbind_typ T ++ E2)        
+.
+
+
+(* Theorem progress.  *)
+
+Lemma d_subenv_same_dom : forall E E', 
+  d_subenv E' E ->
+  dom E = dom E'.
+Proof.
+  intros. induction H; simpl; auto; rewrite IHd_subenv; auto.
+Qed.
+
+Lemma d_subenv_same_tvar : forall E E' X, 
+  d_subenv E' E ->
+  binds X dbind_tvar_empty E ->
+  binds X dbind_tvar_empty E'.
+Proof.
+  intros. induction H; simpl; intros; auto.
+  - inversion H0; auto.
+    + inversion H1; auto.
+  - inversion H0; auto.
+    + inversion H1; auto.
+  - inversion H0; auto.
+    inversion H2.
+Qed.
+
+Lemma d_subenv_same_stvar : forall E E' SX, 
+  d_subenv E' E ->
+  binds SX dbind_stvar_empty E ->
+  binds SX dbind_stvar_empty E'.
+Proof.
+  intros. induction H; simpl; intros; auto.
+  - inversion H0; auto.
+    + inversion H1; auto.
+  - inversion H0; auto.
+    + inversion H1; auto.
+  - inversion H0; auto.
+    inversion H2.
+Qed.
+
+
+Lemma d_subenv_wf_typ : forall E T, 
+  E ⊢ T -> 
+  forall E', 
+    d_subenv E' E ->
+    E' ⊢ T.
+Proof.
+  intros E T H. induction H; intros; auto.
+  - econstructor. 
+    eapply d_subenv_same_tvar; eauto.
+  - econstructor.
+    eapply d_subenv_same_stvar; eauto.
+  - eapply dwftyp_all with (L:=L).
+    + intros. inst_cofinites_with X. auto.
+    + intros. inst_cofinites_with X. eapply H1.
+      econstructor. auto.
+Qed.
+
+
+Lemma d_subenv_wf_env : forall E, 
+  ⊢ E -> 
+  forall E', 
+    d_subenv E' E ->
+    ⊢ E'.
+Proof.
+  intros E H. induction H; intros.
+  - inversion H. auto.
+  - dependent destruction H1.
+    econstructor; auto. 
+    erewrite <- d_subenv_same_dom; auto.
+  - dependent destruction H1.
+    econstructor; auto. 
+    erewrite <- d_subenv_same_dom; auto.
+  - dependent destruction H2.
+    econstructor; auto.
+    + apply dsub_dwft in H3; destruct H3.
+      eapply d_subenv_wf_typ; eauto.
+    + erewrite <- d_subenv_same_dom; auto.
+Qed.
+
+Hint Resolve d_subenv_wf_typ : typing.
+Hint Resolve d_subenv_wf_env : typing.
+Hint Resolve d_wft_typ_subst : typing.
+Hint Resolve d_wf_env_subst_tvar_typ : typing.
+Hint Resolve bind_typ_subst : typing. 
+Hint Resolve dwf_typ_dlc_type : typing.
+
+
+Theorem chkinffinapp_subst: forall E F X e m T1 T2,
+  d_typing (F ++ X ~ dbind_tvar_empty ++ E) e m T1 ->
+  E ⊢ T2 ->
+  dmono_typ T2 ->
+  d_typing (map (d_subst_tv_in_binding T2 X) F  ++ E) (d_subst_tv_in_dexp T2 X e) (d_subst_tv_in_typingmode T2 X m) ({T2 /ᵈ X} T1).
+Proof with auto with typing.
+  intros.
+  generalize dependent T2.
+  dependent induction H; intros; try solve [simpl in *; eauto 5 with typing].
+  - simpl in *. eapply d_typing_inftabs with (L:=L `union` singleton X).
+    + replace (dtyp_all ({T2 /ᵈ X} T1)) with ({T2 /ᵈ X}  dtyp_all T1) by auto.
+      auto... 
+    + intros. specialize (notin_union_1 _ _ _ H4). intros.
+      specialize (H1 _ H5 E (X0 ~ dbind_tvar_empty ++ F) X (JMeq_refl _) T2 H2 H3).
+      assert (lc_dtyp T2) by eauto...
+      specialize (d_subst_tv_in_dexp_open_dexp_wrt_dtyp e T2 (dtyp_var_f X0) X H6).
+      intros. simpl in H7. unfold eq_dec in H7.
+      destruct (EqDec_eq_of_X X0 X) in H7.
+      * subst. apply notin_union_2 in H4. apply notin_singleton_1 in H4.
+        contradiction.
+      * rewrite <- H7. rewrite dtyp_subst_open_comm; auto.
+  - simpl in *. rewrite d_subst_tv_in_dtyp_open_dtyp_wrt_dtyp; eauto...
+  - simpl in *. apply d_typing_chkabstop with (L:=L).
+    intros x Hfr. inst_cofinites_with x.
+    replace (dexp_var_f x) with (d_subst_tv_in_dexp T2 X (dexp_var_f x)) by auto.
+    rewrite <-  d_subst_tv_in_dexp_open_dexp_wrt_dexp. 
+    replace (x ~ dbind_typ dtyp_bot ++ map (d_subst_tv_in_binding T2 X) F ++ E) with 
+    ((map (d_subst_tv_in_binding T2 X) (x ~ dbind_typ dtyp_bot ++ F)) ++ E) by auto. 
+    auto...
+  - simpl in *. eapply d_typing_chkabs with (L:=L); eauto...
+    intros X1 Hfr.
+    inst_cofinites_with X1.
+    specialize (H1 E ((X1, dbind_typ T1) :: F ) X (JMeq_refl _) T0 H2 H3).
+    replace (dexp_var_f X1) with (d_subst_tv_in_dexp T0 X (dexp_var_f X1)) by (simpl; auto).
+    rewrite <- d_subst_tv_in_dexp_open_dexp_wrt_dexp; eauto...
+  - simpl in *. eapply d_typing_chkall with (L:=L `union` singleton X); eauto...
+    + replace (dtyp_all ({T2 /ᵈ X} T1)) with ({T2 /ᵈ X} dtyp_all T1) by auto. 
+      auto...
+    + intros. inst_cofinites_with X0.
+      rewrite dtyp_subst_open_comm; eauto...
+      replace (X0 ~ dbind_tvar_empty ++ map (d_subst_tv_in_binding T2 X) F ++ E) with 
+      (map (d_subst_tv_in_binding T2 X) (X0 ~ dbind_tvar_empty ++ F) ++ E) by auto.
+      auto.
+  - simpl in *. 
+    apply d_typing_chksub with (S1:=({T2 /ᵈ X} S1)); eauto.
+    eapply d_sub_subst_mono; eauto.
+  - simpl in *. eapply d_typing_infappall with (T3:={T0 /ᵈ X} T3); eauto...
+    + apply d_mono_typ_subst_mono_mono; auto.
+    + replace (dtyp_all ({T0 /ᵈ X} T1)) with ({T0 /ᵈ X} dtyp_all T1) by auto.
+      auto...
+    + rewrite <- d_subst_tv_in_dtyp_open_dtyp_wrt_dtyp; eauto...
+Qed.
+
+
+Theorem chkinffinapp_subst_poly: forall E F X e m T1 T2,
+  d_typing (F ++ X ~ dbind_tvar_empty ++ E) e m T1 ->
+  E ⊢ T2 ->
+  d_typing (map (d_subst_tv_in_binding T2 X) F  ++ E) (d_subst_tv_in_dexp T2 X e) (d_subst_tv_in_typingmode T2 X m) ({T2 /ᵈ X} T1).
+Proof with auto with typing.
+  intros.
+  generalize dependent T2.
+  dependent induction H; intros; try solve [simpl in *; eauto 5 with typing].
+  - simpl in *. eapply d_typing_inftabs with (L:=L `union` singleton X).
+    + replace (dtyp_all ({T2 /ᵈ X} T1)) with ({T2 /ᵈ X}  dtyp_all T1) by auto.
+      auto... 
+    + intros. specialize (notin_union_1 _ _ _ H3). intros.
+      specialize (H1 _ H4 E (X0 ~ dbind_tvar_empty ++ F) X (JMeq_refl _) T2 H2).
+      assert (lc_dtyp T2) by eauto...
+      specialize (d_subst_tv_in_dexp_open_dexp_wrt_dtyp e T2 (dtyp_var_f X0) X H5).
+      intros. simpl in H6. unfold eq_dec in H6.
+      destruct (EqDec_eq_of_X X0 X) in H6.
+      * subst. apply notin_union_2 in H3. apply notin_singleton_1 in H3.
+        contradiction.
+      * rewrite <- H6. rewrite dtyp_subst_open_comm; auto.
+  - simpl in *. rewrite d_subst_tv_in_dtyp_open_dtyp_wrt_dtyp; eauto...
+  - simpl in *. apply d_typing_chkabstop with (L:=L).
+    intros x Hfr. inst_cofinites_with x.
+    replace (dexp_var_f x) with (d_subst_tv_in_dexp T2 X (dexp_var_f x)) by auto.
+    rewrite <-  d_subst_tv_in_dexp_open_dexp_wrt_dexp. 
+    replace (x ~ dbind_typ dtyp_bot ++ map (d_subst_tv_in_binding T2 X) F ++ E) with 
+    ((map (d_subst_tv_in_binding T2 X) (x ~ dbind_typ dtyp_bot ++ F)) ++ E) by auto. 
+    auto...
+  - simpl in *. eapply d_typing_chkabs with (L:=L); eauto...
+    intros X1 Hfr.
+    inst_cofinites_with X1.
+    specialize (H1 E ((X1, dbind_typ T1) :: F ) X (JMeq_refl _) T0 H2).
+    replace (dexp_var_f X1) with (d_subst_tv_in_dexp T0 X (dexp_var_f X1)) by (simpl; auto).
+    rewrite <- d_subst_tv_in_dexp_open_dexp_wrt_dexp; eauto...
+  - simpl in *. eapply d_typing_chkall with (L:=L `union` singleton X); eauto...
+    + replace (dtyp_all ({T2 /ᵈ X} T1)) with ({T2 /ᵈ X} dtyp_all T1) by auto. 
+      auto...
+    + intros. inst_cofinites_with X0.
+      rewrite dtyp_subst_open_comm; eauto...
+      replace (X0 ~ dbind_tvar_empty ++ map (d_subst_tv_in_binding T2 X) F ++ E) with 
+      (map (d_subst_tv_in_binding T2 X) (X0 ~ dbind_tvar_empty ++ F) ++ E) by auto.
+      auto.
+  - simpl in *. 
+    apply d_typing_chksub with (S1:=({T2 /ᵈ X} S1)); eauto.
+    admit.
+  - simpl in *. 
+    econstructor.
+  
+  eapply d_typing_infappall with (T3:={T0 /ᵈ X} T3); eauto...
+    + apply d_mono_typ_subst_mono_mono; auto.
+    + replace (dtyp_all ({T0 /ᵈ X} T1)) with ({T0 /ᵈ X} dtyp_all T1) by auto.
+      auto...
+    + rewrite <- d_subst_tv_in_dtyp_open_dtyp_wrt_dtyp; eauto...
+Qed.
+
+
+Fixpoint dexp_size (e : dexp) : nat :=
+  0.
+
+Fixpoint dtyp_size (T : dtyp) : nat :=
+  0.
+
+Definition dmode_size (mode : d_typing_mode) : nat := 
+  match mode with 
+  | d_typingmode_inf => 2
+  | d_typingmode_chk => 1
+  | d_typingmode_infapp _ => 0
+  end.
+
+Definition dmode_type_size (mode : d_typing_mode) : nat := 
+  match mode with 
+  | d_typingmode_inf => 0
+  | d_typingmode_chk => 0
+  | d_typingmode_infapp T =>  dtyp_size T
+  end.
+
+
+Theorem dchk_dinf_dinfapp_subsumption : forall n1 n2 n3 E E' e T mode,
+  dexp_size e < n1 ->
+  dmode_size mode < n2 -> 
+  dtyp_size T + dmode_type_size mode < n3 ->
+  d_typing E e mode T ->
+  d_subenv E' E ->
+    match mode with 
+    | d_typingmode_chk => forall S, E ⊢ T <: S -> d_typing E' e d_typingmode_chk S
+    | d_typingmode_inf => exists S, E ⊢ S <: T /\ d_typing E' e d_typingmode_inf S
+    | d_typingmode_infapp T1 => forall S1, E ⊢ S1 <: T1 -> exists S2, E ⊢ S2 <: T /\ d_typing E' e (d_typingmode_infapp S1) S2
+    end.
+Proof.
+  intro n1; induction n1; intro n2; induction n2; intro n3; induction n3. intros.
+  - admit.
+  - admit.
+  - admit.
+Admitted.
+
+(* Theorem dchk_subsumption : forall e n,
+  dexp_size e < n -> 
+  forall E S,
+    E ⊢ e ⇐ S ->
+    forall  E' T, 
+      d_subenv E' E ->
+      E ⊢ S <: T ->
+      E' ⊢ e ⇐ T
+with 
+dinf_subsumption : forall e n,
+  dexp_size e < n ->
+  forall E T, 
+    E ⊢ e ⇒ T ->
+    forall E',
+      d_subenv E' E ->
+      exists S, 
+        dsub E S T /\ E' ⊢ e ⇒ S
+with 
+dinfapp_subsumption : forall e n, 
+  dexp_size e < n ->
+    forall E T1 T2,  
+    E ⊢ T1 • e ⇒⇒ T2 ->
+    (exists T, E ⊢ e ⇐ T) /\
+    forall E' S1, 
+      d_subenv E' E -> 
+      E ⊢ S1 <: T1 -> 
+      exists S2, 
+        E ⊢ S2 <: T2 /\ E' ⊢ S1 • e ⇒⇒ S2.
+Proof.
+  - intros e n.
+    induction n.
+
+Theorem dchk_subsumption : forall E e S,
+  E ⊢ e ⇐ S ->
+  forall  E' T, 
+    d_subenv E' E ->
+    E ⊢ S <: T ->
+    E' ⊢ e ⇐ T
+with 
+dinf_subsumption : forall E e T, 
+  E ⊢ e ⇒ T ->
+  forall E',
+    d_subenv E' E ->
+    exists S, 
+      dsub E S T /\ E' ⊢ e ⇒ S
+with 
+dinfapp_subsumption : forall E T1 e T2,
+  E ⊢ T1 • e ⇒⇒ T2 ->
+  (exists T, E ⊢ e ⇐ T) /\
+  forall E' S1, 
+    d_subenv E' E -> 
+    E ⊢ S1 <: T1 -> 
+    exists S2, 
+      E ⊢ S2 <: T2 /\ E' ⊢ S1 • e ⇒⇒ S2.
+Proof.
+  - intros E e S H.
+    induction H; auto; intros.
+    + dependent induction H2; eauto.
+    + dependent induction H3. 
+      * apply dchk_top_abs with (L:=L `union` dom E). intros.
+      inst_cofinites_with x.
+      dependent destruction H3.
+      apply H1; auto.
+      econstructor; auto.
+      constructor.
+      admit. (* easy: weakening *)
+      * eapply dchk_abs with (L:=L).
+        -- eauto.  apply dsub_dwft in H3_.
+           apply dsub_dwft in H3_0.
+           destruct H3_. destruct H3_0.
+           eauto.
+        -- intros. inst_cofinites_with x.  
+          apply H1. econstructor; eauto.
+          admit. (* easy: weakening *)
+      * apply dchk_intersection; eauto.
+      * apply dchk_union1; eauto. 
+      * apply dchk_union2; eauto.
+    + specialize (dinf_subsumption _ _ _ H _ H1).
+      destruct dinf_subsumption as [S1 [Hsub Hinf]].
+      specialize (dinfapp_subsumption _ _ _ _ H0 ).
+      destruct dinfapp_subsumption as [Hchk Hinfapp_subsumption].
+      specialize (Hinfapp_subsumption _ _ H1 Hsub).
+      destruct Hinfapp_subsumption as [S2 [Hsub2 Hinfapp]].
+      eapply dchk_sub with (S:=S2).
+      eapply dinf_app with (T2:=S1); auto.
+      admit. (* easy : transitivity *)
+    (* e <= ∀ X. T *)
+    + admit.
+    (* e <= T *)
+    + specialize (dinf_subsumption _ _ _ H _ H1).
+      destruct dinf_subsumption as [S1 [Hsub Hinf]].
+      eapply dchk_sub; eauto. 
+      admit. (* easy : transitivity *)
+    (* e <= S * T *)
+    + dependent induction H2.
+      * dependent destruction H2. eapply dchk_subsumption; eauto.
+      * eapply dchk_intersection.
+        -- eapply IHdsub1 with (S:=S) (T:=T); eauto.
+        -- eapply IHdsub2 with (S:=S) (T:=T); eauto.
+      * eapply IHdchk1; eauto.
+      * eapply IHdchk2; eauto.
+      * eapply dchk_union1. eapply IHdsub with (S:=S) (T:=T); eauto.
+        eauto.
+      * eapply dchk_union2. eapply IHdsub with (S:=S) (T:=T); eauto.
+        eauto.
+    (* e <= S + T *)
+    + apply dsub_union_inversion in H2. destruct H2.
+      auto.
+    (* e <= S + T *)
+    + apply dsub_union_inversion in H2. destruct H2.
+      auto.
+
+  - intros. induction H.
+    + admit. (* easy *)
+    + exists T. split; auto.
+      * apply dsub_refl; auto.
+      * apply dinf_anno.
+        eapply d_subenv_wf_typ; eauto.
+        eapply dchk_subsumption; eauto.
+        apply dsub_refl; auto.
+    + eauto.
+      (* exists dtyp_unit.
+      split; eauto.  *)
+    + eauto. 
+      (* + specialize (dinfapp_subsumption _ _ _ _ H1).
+      destruct dinfapp_subsumption as [Hchk Hinfapp_subsumption].
+      specialize (IHdinf H0).
+      destruct IHdinf as [S1 [Hsub Hinf]].
+      specialize (Hinfapp_subsumption _ _ H0 Hsub).
+      destruct Hinfapp_subsumption as [S2 [Hsub1 Hinfapp]].
+      exists S2. split; eauto. *)
+    (* e => ∀ X. T *)
+    + admit.
+    + specialize (IHdinf H0).
+      destruct IHdinf as [S1 [Hsub Hinf]].
+      dependent induction Hsub; eauto.
+    + admit.
+    
+  - intros; induction H.
+    + split. exists T1. auto. 
+      intros. dependent induction H2; auto.
+      * dependent destruction H2. exists dtyp_bot; split;     eauto. 
+      * exists S2; split; eauto.
+        constructor; eauto. admit.
+      * admit.
+      * specialize (IHdsub _ _ H H0 H1 (eq_refl _)).
+        destruct IHdsub as [S3 [Hsub Hinfapp]].
+        exists S3; split; auto. 
+        admit. (* TODO : check rule *)
+      * specialize (IHdsub _ _ H H0 H1 (eq_refl _)).
+        destruct IHdsub as [S3 [Hsub Hinfapp]].
+        exists S3; split; auto. 
+        admit. (* TODO : check rule *)
+      * admit. (* TODO : check rule *)
+    + destruct IHdinfapp as [Hchk Hinfapp].
+      destruct Hchk as [T]. split.
+      exists T; auto. 
+      intros. dependent induction H5.
+      * exists dtyp_bot; split.
+        -- constructor. admit.
+        -- econstructor. eapply dchk_subsumption; eauto.
+            econstructor. admit. 
+      * admit.
+      * admit.
+      * admit.
+      * admit.
+      * admit.
+
+    + split.
+      exists dtyp_top; auto. 
+      intros. dependent induction H1.
+      * exists dtyp_bot. split; eauto.
+      * specialize (IHdsub H H0 (eq_refl _)).
+        destruct IHdsub as [S2 [Hsub Hinfapp]].
+        exists S2; split; eauto.
+        econstructor; eauto. admit.
+      * admit. (* TODO : check rule *)
+      * admit. (* TODO : check rule *)  
+      * admit. (* TODO : check rule *)  
+Admitted.
+ *)
